\documentclass[handout]{ximera}
%\documentclass[10pt,handout,twocolumn,twoside,wordchoicegiven]{xercises}
%\documentclass[10pt,handout,twocolumn,twoside,wordchoicegiven]{xourse}

\input{../../preamble.tex}

\outcome{Practice Limits.}
   

\title{Limits with infinity practice}

\begin{document}
\begin{abstract}
Here is an opportunity for you to practice evaluating limits that involve infinity.  
\end{abstract}
\maketitle

%% Vertical Asymptote 1
\begin{exercise}
Your goal in this exercise is to evaluate $\displaystyle\lim_{x \to -3} \frac{1}{(x+3)^3}$ (if it exists).  First, consider the corresponding one-sided limits:

$$\lim_{x \to -3^-} \frac{1}{(x+3)^3} \text{ and } \lim_{x \to -3^+} \frac{1}{(x+3)^3}.$$

As $x$ approaches $-3$ from the left:  

\begin{itemize}

\item The function $1$ approaches $\answer{1}$, which is a \wordChoice{\choice[correct]{positive}\choice{negative}} number. 

\item $(x+3)^3$ approaches a small \wordChoice{\choice{positive}\choice[correct]{negative}} number. 

\end{itemize}

Therefore, 

 \[ \lim_{x \to -3^-} \frac{1}{(x+3)^3} = \answer{-\infty}.\]
 
As $x$ approaches $-3$ from the right: 

\begin{itemize}

\item The function $1$ approaches $\answer{1}$, which is a \wordChoice{\choice[correct]{positive}\choice{negative}} number. 

\item $(x+3)^3$ approaches a small \wordChoice{\choice[correct]{positive}\choice{negative}} number. 

\end{itemize}

Therefore, 

 \[ \lim_{x \to -3^+} \frac{1}{(x+3)^3} = \answer{\infty}. \]

Putting all of this information together, you can conclude that

\[ \lim_{x \to -3} \frac{1}{(x+3)^3} = \answer{DNE}. \]

\begin{exercise}

From the above limit calculations, you can say that $\frac{1}{(x+3)^3}$ \wordChoice{\choice[correct]{does}\choice{does not}} have a \wordChoice{\choice{horizontal}\choice[correct]{vertical}} asymptote at $x =-3$. 

\end{exercise}

\end{exercise}

%% Vertical Asymptote 2
\begin{exercise}
Your goal in this exercise is to evaluate $\displaystyle\lim_{x \to 7} \frac{-3x+2}{(x-7)^6}$ (if it exists).  First, consider the corresponding one-sided limits:

$$\displaystyle\lim_{x \to 7^-} \frac{-3x+2}{(x-7)^6} \text{ and } \displaystyle\lim_{x \to 7^+} \frac{-3x+2}{(x-7)^6}.$$

As $x$ approaches $7$ from the left:  

\begin{itemize}

\item The function $-3x+2$ approaches $\answer{-19}$, which is a \wordChoice{\choice{positive}\choice[correct]{negative}} number. 

\item $(x-7)^6$ approaches a small \wordChoice{\choice[correct]{positive}\choice{negative}} number. 

\end{itemize}

Therefore, 

 \[ \displaystyle\lim_{x \to 7^-} \frac{-3x+2}{(x-7)^6} = \answer{-\infty}.\]
 
As $x$ approaches $7$ from the right: 

\begin{itemize}

\item The function $-3x+2$ approaches $\answer{-19}$, which is a \wordChoice{\choice{positive}\choice[correct]{negative}} number. 

\item $(x-7)^6$ approaches a small \wordChoice{\choice[correct]{positive}\choice{negative}} number. 

\end{itemize}

Therefore, 

 \[ \displaystyle\lim_{x \to 7^+} \frac{-3x+2}{(x-7)^6} = \answer{-\infty}. \]

Putting all of this information together, you can conclude that

\[ \displaystyle\lim_{x \to 7} \frac{-3x+2}{(x-7)^6} = \answer{-\infty}. \]

\begin{exercise}

From the above limit calculations, you can say that $\frac{-3x+2}{(x-7)^3}$ \wordChoice{\choice[correct]{does}\choice{does not}} have a \wordChoice{\choice{horizontal}\choice[correct]{vertical}} asymptote at $x =7$. 

\end{exercise}

\end{exercise}

%% Vertical Asymptote 3
\begin{exercise}

Consider the function $f(x) = \frac{x^2+x-6}{x^2-3x+2}$.  The two $x$-values at which $f(x)$ may have a vertical asymptote are

\begin{hint}
On this problem, it will help to factor the numerator and denominator of $f(x)$.

\end{hint}

\begin{multipleChoice}
    \choice{$x = -2, 6$}
    \choice[correct]{$x = 1, 2$}
    \choice{$x = -3, 1$}
    \choice{$x = 2, -3$}
    
    \begin{feedback}[correct]
    Good thinking!  For a rational function like $f(x)$, there could be an asymptote at all the $x$ values where $f$ is undefined.  The only way for $f$ to be undefined is if the denominator of $f$ is 0.  Since $x^2 -3x + 2 = (x-1)(x-2)$, the $x$ values that make the denominator 0 are $x = 1, 2$, so these are the potential values at which $f$ may have a vertical asymptote. 
    \end{feedback}
\end{multipleChoice}
    
\begin{exercise}
Now, determine if $x = 1$ and $x = 2$ are asymptotes of $f$ or not. 

As $x$ approaches $1$ from the left:  

\begin{itemize}

\item The function $x^2 + x -6$ approaches $\answer{-4}$, which is a \wordChoice{\choice{positive}\choice[correct]{negative}} number. 

\item $x^2 - 3x + 2$ approaches a small \wordChoice{\choice[correct]{positive}\choice{negative}} number.

\end{itemize}

Therefore, 

\[ \displaystyle\lim_{x \to 1^-} \frac{x^2+x-6}{x^2-3x+2} = \answer{-\infty} \]

and based on this limit information, you can conclude that

\begin{multipleChoice}
    \choice[correct]{$x = 1$ is a vertical asymptote of $f$.}
    \choice{$x = 1$ is not a vertical asymptote of $f$.}
    \choice{$x = 1$ may or may not be a vertical asymptete of $f$.  There isn't enough information to decide yet.}
\end{multipleChoice}

\begin{exercise}
Alright, now you know that $x=1$ is a vertical asymptote of $f$.  What about $x=2$?  Well, 

\[ \displaystyle\lim_{x \to 2^-} \frac{x^2+x-6}{x^2-3x+2} = \answer{5} \]

and based on this limit information, you can conclude that

\begin{multipleChoice}
    \choice{$x = 2$ is a vertical asymptote of $f$.}
    \choice{$x = 2$ is not a vertical asymptote of $f$.}
    \choice[correct]{$x = 2$ may or may not be a vertical asymptote of $f$.  There isn't enough information to decide yet.}
\end{multipleChoice}

\begin{exercise}
Because the limit information we have so far isn't enough to make any conclusions, evaluate the other one-sided limit: 

\[ \displaystyle\lim_{x \to 2^+} \frac{x^2+x-6}{x^2-3x+2} = \answer{5}. \]

\begin{exercise}

Now, from all information you have obtained about the limit of $f(x)$ at $x=2$, you can conclude that 

\begin{multipleChoice}
    \choice{$x = 2$ is a vertical asymptote of $f$.}
    \choice[correct]{$x = 2$ is not a vertical asymptote of $f$.}
    \choice{$x = 2$ may or may not be a vertical asymptote of $f$.  There isn't enough information to decide yet.}
    
    \begin{feedback}[correct]
    It turns out that $\displaystyle\lim_{x \to 2} \frac{x^2+x-6}{x^2-3x+2} = 5$ while $f(2)$ does not exist.  This indicates that there is a hole at $x=2$ and not a vertical asymptote!  In fact, if you factor $f(x)$, you'll realize that a factor of $(x-2)$ appears precisely once in the numerator and denominator.  Because of this, when you evaluate $\displaystyle\lim_{x \to 2} \frac{x^2+x-6}{x^2-3x+2}$, the $(x-2)$'s will cancel out, and you'll find that the limit exists.  This kind of 'cancellation set-up' is a tell-tale sign that the function at hand has a hole at $x=2$ rather than a vertical asymptote.  
    \end{feedback}
    
\end{multipleChoice}

\end{exercise}

\end{exercise}

\end{exercise}

\end{exercise}

\end{exercise}


\begin{exercise}

Evaluate the limit. 

\[ \displaystyle\lim_{x \to \infty} \frac{3x +7 - x^5}{x^4 + 8x^2 -3} = \answer{-\infty} \]

\begin{exercise}

To evaluate the above limit, you had to multiply the numerator and denominator of $\frac{3x +7 - x^5}{x^4 + 8x^2 -3}$ by $\cfrac{1}{x^{\answer{4}}}.$

\end{exercise}

\end{exercise}

\begin{exercise}

Evaluate the limit. 

\[ \displaystyle\lim_{x \to -\infty} \frac{x^6 + 3.5x^3 -70x^2 + 2\pi}{3x - \frac{1}{3}x^3+ 4x^6} = \answer{-\infty} \]

\begin{exercise}

To evaluate the above limit, you had to multiply the numerator and denominator of $\frac{5x^6 + 3.5x^3 -70x^2 + 2\pi}{3x - \frac{1}{3}x^3+ 4x^6}$ by $\cfrac{1}{x^{\answer{\frac{5}{6}}}}.$

\end{exercise}

\end{exercise}





\end{document}
